init recLIS

dp/lis.dfy
@@ -1,7 +1,16 @@
 include "../prop.dfy"
 
-//https://classroom.udacity.com/courses/ud401/lessons/9752571100/concepts/98020206310923
-predicate recLIS(l: seq<nat>, a: seq<int>)
+function maxLIS(l: seq<nat>, a: seq<int>, val: int): int
+decreases l, a
+requires |l| == |a| > 0
 {
-    false
+    if |l| == 1 || |a| == 1 then l[|l|-1] else
+    if l[|l|-1] == Prop.calcMax(l) && val >= a[|a|-1] then l[|l|-1]
+    else maxLIS(l[..|l|-1], a[..|a|-1], val)
+}
+
+predicate recLIS(l: seq<nat>, a: seq<int>)
+requires |l| == |a| > 0
+{
+    forall i, j :: 1 <= j <= i-1 < |l|-1 && a[j] < a[i] ==> l[i] == 1 + maxLIS(l[..j], a[..j], a[j])
 }
